Some progress, or something

theories/vir/mcfg_contextual.v
@@ -7,7 +7,8 @@ From velliris.vir Require Import
 From Vellvm Require Import Syntax.DynamicTypes Handlers Syntax.LLVMAst
   Semantics.InterpretationStack.
 
-From ITree Require Import Recursion.
+From ITree Require Import ITree Recursion.
+From Equations Require Import Equations.
 
 Import LLVMEvents.
 
@@ -17,21 +18,505 @@ Section mcfg_contextual.
 
   Context `(sheapGS Σ, checkedoutGS Σ, heapbijGS Σ).
 
+  Definition frame_inv i_t i_s :=
+    (frame_WF i_t i_s ∗ checkout ∅ ∗ stack_tgt i_t ∗ stack_src i_s)%I.
+
+  (* An obligation for each of the defined calls; it satisfies the external
+      call specifications *)
+  Definition context_rel_call_inv
+      (f : ∀ T : Type, CallE T → L0'expr T)
+      (g : ∀ T : Type, CallE T → L0'expr T) :=
+    (□ (∀ fn1 fn2 dt1 dt2 attr1 attr2 args1 args2 C,
+          let call1 := ExternalCall dt1 fn1 args1 attr1 in
+          let call2 := ExternalCall dt2 fn2 args2 attr2 in
+          call_ev call1 call2 C -∗
+          ⟅ f _ (Call dt1 fn1 args1 attr1) ⟆ ⪯
+          ⟅ g _ (Call dt2 fn2 args2 attr2) ⟆
+          [[ (fun v1 v2 => call_ans call1 v1 call2 v2 C) ⤉ ]]) )%I.
+
+  (* Should follow by reflexivity theorem *)
+  Definition context_rel_refl
+      (f : ∀ T : Type, CallE T → L0'expr T)
+      (g : ∀ T : Type, CallE T → L0'expr T) :=
+    (□ (∀ fn1 fn2 dt attr args1 args2 C,
+          arg_val_rel (fn1, args1) (fn2, args2) C -∗
+          ⟅ f _ (Call dt fn1 args1 attr) ⟆ ⪯
+          ⟅ g _ (Call dt fn2 args2 attr) ⟆
+          [[ (fun x y => res_val_rel x y C) ⤉ ]]))%I.
+
+  (* Definition context_call *)
+  (*     (f : ∀ T : Type, CallE T → L0'expr T) := *)
+  (*   (forall τ addr args attrs, *)
+  (*     f uvalue (Call τ addr args (FNATTR_Internal :: attrs)) = *)
+  (*     f uvalue (Call τ addr args attrs)) /\ *)
+  (*   (forall τ addr args attrs, *)
+  (*     f uvalue (Call τ addr args (FNATTR_External:: attrs)) = *)
+  (*     f uvalue (Call τ addr args attrs)). *)
+
+  Definition context_rel
+      (f : ∀ T : Type, CallE T → L0'expr T)
+      (g : ∀ T : Type, CallE T → L0'expr T) :=
+    (context_rel_call_inv f g ∗ context_rel_refl f g)%I.
+
+  Theorem Proper_interp_mrec' {R}
+    (f g : ∀ T : Type, LLVMEvents.CallE T → L0'expr T) a1 a2
+    (Ψ : R -d> R -d> iPropI Σ) i_t i_s :
+    frame_inv i_t i_s -∗
+    context_rel f g -∗
+    <pers>
+    (frame_inv i_t i_s -∗ ⟅ a1 ⟆ ⪯ ⟅ a2 ⟆ [[ (fun x y => Ψ x y ∗ frame_inv i_t i_s) ⤉ ]]) -∗
+    interp_mrec f a1 ⪯ interp_mrec g a2
+    [[ (fun x y => Ψ x y ∗ frame_inv i_t i_s) ⤉ ]].
+  Proof.
+    iIntros "Hinv Hrel #Hr".
+    iSpecialize ("Hr" with "Hinv").
+  Admitted.
+
+  (* Type declaration for function definitions, i.e. an association list for
+     function definitions with [dvalue] keys. *)
+  Definition fundefs : Type := list (dvalue * definition dtyp (CFG.cfg dtyp)).
+
+  Definition fundef_no_attr (def : definition dtyp (CFG.cfg dtyp)) :=
+    RelDec.rel_dec (dc_attrs (df_prototype def)) nil.
+
+  (* The function definition map [fd] does not have any attributes at its
+    definition site. *)
+  Definition fundefs_no_attr (fd : fundefs) :=
+    forallb (fun '(_, def) => fundef_no_attr def) fd.
+
+  Lemma sim_external_call dτ addr_t addr_s args_t args_s l i_t i_s:
+    frame_WF i_t i_s -∗
+    stack_tgt i_t -∗
+    stack_src i_s -∗
+    checkout ∅ -∗
+    dval_rel addr_t addr_s -∗
+    ([∗ list] x;y ∈ args_t;args_s, uval_rel x y) -∗
+    ⟅ dargs <- Util.map_monad (λ uv : uvalue, pickUnique uv) args_t;;
+    trigger (ExternalCall dτ addr_t (map dvalue_to_uvalue dargs) l) ⟆
+    ⪯
+    ⟅ dargs <- Util.map_monad (λ uv : uvalue, pickUnique uv) args_s;;
+    trigger (ExternalCall dτ addr_s (map dvalue_to_uvalue dargs) l) ⟆
+    [[ (fun x y =>
+    uval_rel x y ∗ stack_tgt i_t ∗ stack_src i_s ∗
+    checkout ∅) ⤉ ]].
+  Proof. Admitted.
+
   (* The contextual refinement on [denote_mcfg]. *)
   Lemma contextual_denote_mcfg :
     ∀ γ_t γ_s dv dv' e_t e_s main C,
+    fundefs_no_attr C ->
+    fundef_no_attr e_t ->
+    fundef_no_attr e_s ->
     □ fun_logrel e_t e_s ∅ -∗
       checkout ∅ -∗
       stack_tgt [γ_t] -∗
       stack_src [γ_s] -∗
+      dval_rel dv dv' -∗
+      ([∗ list] v_t;v_s ∈ C.*1;C.*1, dval_rel v_t v_s) -∗
       denote_mcfg ((dv, e_t) :: C) DTYPE_Void (DVALUE_Addr main) []
       ⪯
       denote_mcfg ((dv', e_s) :: C) DTYPE_Void (DVALUE_Addr main) []
       [[ (λ x y : uvalue, ⌜obs_val x y⌝) ⤉ ]].
   Proof.
-    iIntros (????????) "#Hfun Hc Hs_t Hs_s".
+    iIntros (???????? HC H_t H_s) "#Hfun Hc Hs_t Hs_s #Hdv #Hfun_keys".
     rewrite /denote_mcfg.
 
-  Admitted.
+    iAssert (frame_inv [γ_t] [γ_s])%I with "[Hc Hs_t Hs_s]" as "Hinv".
+    { by iFrame. }
 
-End mcfg_contextual.
+    iPoseProof
+      (Proper_interp_mrec' _ _ _ _ (λ x y : uvalue, ⌜obs_val x y⌝)%I [γ_t] [γ_s]
+        with "Hinv") as "Hrec"; eauto.
+    iApply (sim_expr'_bupd_mono with "[] [Hrec]"); last iApply "Hrec".
+    { iIntros (??) "HΨ"; iDestruct "HΨ" as (????) "(%HΨ & HI)".
+      iExists _, _; iFrame. done. }
+
+    { rewrite /context_rel.
+
+      iSplitL ""; cycle 1.
+      {  (* REFL *)
+        iIntros (??).
+        iModIntro.
+        iIntros (?????).
+        destruct C0 as ((?&?)&?).
+        rewrite /arg_val_rel. cbn -[denote_function].
+        iIntros "Hev".
+        iDestruct "Hev" as "(#HWF & HC & Hst & Hss & #Hfn & #Hargs)".
+        subst.
+
+        destruct (lookup_defn fn2 ((dv', e_s) :: C)) eqn: Hs; cycle 1.
+
+        (* External call case *)
+        { cbn in Hs. destruct_if; reldec.
+          iDestruct (dval_rel_ne_inj with "Hfn Hdv") as %Hne.
+          assert (dv' <> fn2) by eauto.
+          specialize (Hne H3). cbn -[denote_function].
+          destruct (RelDec.rel_dec fn1 dv) eqn: Hfn1; reldec; try done.
+          iPoseProof (dval_rel_lookup_none with "Hfn Hfun_keys") as "%Hlu".
+          rewrite /lookup_defn.
+          specialize (Hlu Hs); rewrite Hlu.
+
+          rewrite /call_ev; cbn; simp vir_call_ev.
+          rewrite /lookup_defn in Hs. rewrite Hs.
+
+          iApply (sim_expr'_bupd_mono);
+            last iApply (sim_external_call with "HWF Hst Hss HC Hfn Hargs").
+          iIntros (??) "H'".
+          rewrite /lift_post.
+          iDestruct "H'" as (????) "(#Hv' & HC & Hs_t & Hs_s)".
+          iExists _, _; iFrame.
+          repeat (iSplitL ""; first done).
+          simp vir_call_ans; by iFrame. }
+
+        (* Internal call case *)
+        { rewrite /fundefs_rel_WF.
+
+          apply lookup_defn_cons_Some in Hs.
+          destruct Hs.
+          (* It is the [e_s] function (the hole) *)
+          { destruct H2; subst; cbn -[denote_function].
+            iDestruct (dval_rel_inj with "Hdv Hfn") as %Hdef; subst.
+            destruct (RelDec.rel_dec fn1 fn1) eqn: Hf; reldec; subst; last done.
+            destruct (RelDec.rel_dec dv' dv') eqn: Hf'; reldec; subst; last done.
+            subst.
+
+            iDestruct "HWF" as %HWF; subst.
+            rewrite /fundef_no_attr in H_t, H_s.
+            assert (attr = nil).
+            { admit. }
+            rewrite H2.
+            destruct (RelDec.rel_dec (dc_attrs (df_prototype d)) []); try done.
+            destruct (RelDec.rel_dec (dc_attrs (df_prototype e_t)) []); try done.
+
+            iSpecialize ("Hfun" $! _ _ _ _ HWF with "Hst Hss Hargs HC").
+            iApply sim_expr'_bupd_mono; last (iApply "Hfun").
+            iIntros (??) "H'".
+            rewrite /lift_post.
+            iDestruct "H'" as (????) "(Hs_t & Hs_s & HC & Hval)".
+            iExists _, _; iFrame. subst; iModIntro.
+            repeat (iSplitL ""; first done).
+            simp vir_call_ans; by iFrame. }
+
+          (* It is a function in the context *)
+          { destruct H2. cbn -[denote_function].
+
+            iDestruct (dval_rel_ne_inj with "Hdv Hfn") as "%Hne"; subst.
+            specialize (Hne H2); subst.
+            destruct (RelDec.rel_dec fn1 dv) eqn: Hf; reldec; subst; first done.
+            destruct (RelDec.rel_dec fn2 dv') eqn: Hf'; reldec; subst; first done.
+            clear H2 Hne Hf.
+            iPoseProof (dval_rel_lookup_some with "Hfn Hfun_keys") as "%Hlu".
+            specialize (Hlu _ H3). destruct Hlu as (?&?).
+            rewrite /lookup_defn in H3.
+            rewrite /lookup_defn; rewrite H2 H3.
+
+            (* Juicing out information from the WF of fundefs *)
+            unfold fundefs_WF in WF_s.
+            apply andb_prop_elim in WF_s.
+            destruct WF_s as (Hlen & Wdup_s).
+            apply andb_prop_elim in Hlen. destruct Hlen as (Hlen & Hfun_wf).
+            apply forallb_True in Hfun_wf.
+            rewrite List.Forall_forall in Hfun_wf.
+            assert (Hr_s := H3).
+            apply lookup_defn_Some_In in H3.
+            (* Function [d] is well-formed. *)
+            specialize (Hfun_wf _ H3); cbn in Hfun_wf.
+
+            (* Using [fundefs_logrel] *)
+            assert (Hlen': (length [γf0] > 0)%Z → (length [γf] > 0)%Z) by auto.
+            rewrite /fundefs_logrel. rewrite /lookup_defn in Hr_s.
+            apply lookup_defn_Some_lookup in Hr_s.
+            destruct Hr_s.
+            (* Juice information out of fundef rel WF *)
+            iDestruct "Hrel" as "(Hrel & Hn)".
+            iSpecialize ("Hrel" $! _ _ _ H6).
+            iDestruct "Hrel" as (???) "(#Hdv' & %Hattr & %Hattr' & %Hft & %Hfs)".
+
+            iDestruct (dval_rel_inj with "Hfn Hdv'") as %Hf; subst.
+
+            iSpecialize ("Hlr" $! _ _ _ _ _ _ H7 H6 Hattr Hattr'
+                          with "Hdv'").
+            iDestruct "HWF" as %HWF.
+            iSpecialize ("Hlr" $! _ _ _ _ HWF with "Hst Hss Hargs HC").
+
+            eapply lookup_defn_Some in H2; eauto;cycle 1.
+            { clear -WF_t.
+
+              unfold fundefs_WF in WF_t.
+              apply andb_prop_elim in WF_t.
+              destruct WF_t as (Hlen & Wdup_t).
+              apply andb_prop_elim in Hlen. destruct Hlen as (Hlen & Hfun_wf).
+              apply forallb_True in Hfun_wf.
+              rewrite List.Forall_forall in Hfun_wf.
+              apply Is_true_true_1 in Wdup_t.
+              by apply NoDup_b_NoDup. }
+            subst.
+
+            iApply sim_expr'_bupd_mono; last iApply "Hlr".
+            iIntros (??) "Hin".
+            iDestruct "Hin" as (????) "(Hst & Hss & HC & Hval)".
+            iExists _, _.
+            repeat (iSplitL ""; first done).
+            simp vir_call_ans; subst; by iFrame. } } }
+
+      { (* CALL INV *)
+        iIntros (??).
+        iModIntro.
+        iIntros (???????).
+        destruct C0 as ((?&?)&?).
+        rewrite /call_ev. cbn -[denote_function].
+        iIntros "Hev". simp vir_call_ev.
+        iDestruct "Hev" as
+          "(#Hfn &%Hdt & %Hattr& #Hargs & HC & #HWF & Hst & Hss & %Hinterp)".
+        subst.
+
+        destruct (lookup_defn fn2 ((dv', e_s) :: r_s))
+          eqn: Hs; cycle 1.
+
+        (* External call case *)
+        { cbn in Hs. destruct_if; reldec.
+          iDestruct (dval_rel_ne_inj with "Hfn Hdv") as %Hne.
+          assert (dv' <> fn2) by eauto.
+          specialize (Hne H3). cbn -[denote_function].
+          destruct (RelDec.rel_dec fn1 dv) eqn: Hfn1; reldec; try done.
+          iPoseProof (dval_rel_lookup_none with "Hfn Hv") as "%Hlu".
+          rewrite /lookup_defn.
+          specialize (Hlu Hs); rewrite Hlu.
+
+          rewrite /call_ev; cbn; simp vir_call_ev.
+          rewrite /lookup_defn in Hs. rewrite Hs.
+
+          specialize (WF_attr _ _ _ _ _ _ _ _ Hinterp); subst.
+
+          iApply (sim_expr'_bupd_mono);
+            last iApply (sim_external_call with "HWF Hst Hss HC Hfn Hargs").
+          iIntros (??) "H'".
+          rewrite /lift_post.
+          iDestruct "H'" as (????) "(#Hv' & HC & Hs_t & Hs_s)".
+          iExists _, _; iFrame.
+          repeat (iSplitL ""; first done).
+          simp vir_call_ans; by iFrame. }
+
+        (* Internal call case *)
+        { rewrite /fundefs_rel_WF.
+
+          apply lookup_defn_cons_Some in Hs.
+          destruct Hs.
+          (* It is the [e_s] function (the hole) *)
+          { destruct H2; subst; cbn -[denote_function].
+            iDestruct (dval_rel_inj with "Hdv Hfn") as %Hdef; subst.
+            destruct (RelDec.rel_dec fn1 fn1) eqn: Hf; reldec; subst; last done.
+            destruct (RelDec.rel_dec dv' dv') eqn: Hf'; reldec; subst; last done.
+            subst.
+
+            iDestruct "HWF" as %HWF; subst.
+            iDestruct ("Hf" $! _ _ _) as "(_ & Hf')".
+            specialize (WF_attr _ _ _ _ _ _ _ _ Hinterp); subst.
+
+            iSpecialize ("Hf'" $! _ _ _ _ HWF with "Hst Hss Hargs HC").
+            iApply sim_expr'_bupd_mono; last (iApply "Hf'").
+            iIntros (??) "H'".
+            rewrite /lift_post.
+            iDestruct "H'" as (????) "(Hs_t & Hs_s & HC & Hval)".
+            iExists _, _; iFrame. subst; iModIntro.
+            repeat (iSplitL ""; first done).
+            simp vir_call_ans; by iFrame. }
+
+          (* It is a function in the context *)
+          { destruct H2. cbn -[denote_function].
+
+            iDestruct (dval_rel_ne_inj with "Hdv Hfn") as "%Hne"; subst.
+            specialize (Hne H2); subst.
+            destruct (RelDec.rel_dec fn1 dv) eqn: Hf; reldec; subst; first done.
+            destruct (RelDec.rel_dec fn2 dv') eqn: Hf'; reldec; subst; first done.
+            clear H2 Hne Hf.
+            iPoseProof (dval_rel_lookup_some with "Hfn Hv") as "%Hlu".
+            specialize (Hlu _ H3). destruct Hlu as (?&?).
+            rewrite /lookup_defn in H3.
+            rewrite /lookup_defn; rewrite H2 H3.
+
+            (* Juicing out information from the WF of fundefs *)
+            unfold fundefs_WF in WF_s.
+            apply andb_prop_elim in WF_s.
+            destruct WF_s as (Hlen & Wdup_s).
+            apply andb_prop_elim in Hlen. destruct Hlen as (Hlen & Hfun_wf).
+            apply forallb_True in Hfun_wf.
+            rewrite List.Forall_forall in Hfun_wf.
+            assert (Hr_s := H3).
+            apply lookup_defn_Some_In in H3.
+            (* Function [d] is well-formed. *)
+            specialize (Hfun_wf _ H3); cbn in Hfun_wf.
+
+            (* Using [fundefs_logrel] *)
+            assert (Hlen': (length [γf0] > 0)%Z → (length [γf] > 0)%Z) by auto.
+            rewrite /fundefs_logrel. rewrite /lookup_defn in Hr_s.
+            apply lookup_defn_Some_lookup in Hr_s.
+            destruct Hr_s.
+            (* Juice information out of fundef rel WF *)
+            iDestruct "Hrel" as "(Hrel & Hn)".
+            iSpecialize ("Hrel" $! _ _ _ H6).
+            iDestruct "Hrel" as (???) "(#Hdv' & %Hattr & %Hattr' & %Hft & %Hfs)".
+
+            iDestruct (dval_rel_inj with "Hfn Hdv'") as %Hf; subst.
+
+            specialize (WF_attr _ _ _ _ _ _ _ _ Hinterp); subst.
+            iSpecialize ("Hlr" $! _ _ _ _ _ _ H7 H6 Hattr Hattr'
+                          with "Hdv'").
+            iDestruct "HWF" as %HWF.
+            iSpecialize ("Hlr" $! _ _ _ _ HWF with "Hst Hss Hargs HC").
+
+            eapply lookup_defn_Some in H2; eauto;cycle 1.
+            { clear -WF_t.
+
+              unfold fundefs_WF in WF_t.
+              apply andb_prop_elim in WF_t.
+              destruct WF_t as (Hlen & Wdup_t).
+              apply andb_prop_elim in Hlen. destruct Hlen as (Hlen & Hfun_wf).
+              apply forallb_True in Hfun_wf.
+              rewrite List.Forall_forall in Hfun_wf.
+              apply Is_true_true_1 in Wdup_t.
+              by apply NoDup_b_NoDup. }
+            subst.
+
+            iApply sim_expr'_bupd_mono; last iApply "Hlr".
+            iIntros (??) "Hin".
+            iDestruct "Hin" as (????) "(Hst & Hss & HC & Hval)".
+            iExists _, _.
+            repeat (iSplitL ""; first done).
+            simp vir_call_ans; subst; by iFrame. } } } }
+
+    (* Other obligation that "feels like a duplicate obligation",
+    but is a separate one coming from the body of the [mrec] *)
+    { iModIntro. iIntros "(#HWF & HC & Hst & Hss)".
+
+      iAssert (dval_rel (DVALUE_Addr main) (DVALUE_Addr main))%I as "#Hmain".
+      { rewrite (dval_rel_unfold (DVALUE_Addr _)).
+        cbn. iSplitL ""; try done.
+        iDestruct "Haddr_main" as "(Haddr_main & _)"; done. }
+
+      destruct (lookup_defn (DVALUE_Addr main) ((dv', e_s) :: r_s))
+        eqn: Hs; cycle 1.
+
+      (* External call case *)
+      { cbn in Hs. destruct_if; reldec.
+        iDestruct (dval_rel_ne_inj with "Hmain Hdv") as %Hne.
+        assert (dv' <> DVALUE_Addr main) by eauto.
+        specialize (Hne H3). cbn -[denote_function map_monad].
+        destruct (RelDec.rel_dec (DVALUE_Addr main) dv) eqn: Hfn1;
+          reldec; try done.
+        iPoseProof (dval_rel_lookup_none with "Hmain Hv") as "%Hlu".
+        rewrite /lookup_defn.
+        specialize (Hlu Hs); rewrite Hlu.
+
+        iApply (sim_expr'_bupd_mono);
+          last iApply (sim_external_call with "HWF Hst Hss HC Hmain"); try done.
+        iIntros (??) "H'".
+        rewrite /lift_post.
+        iDestruct "H'" as (????) "(#Hv' & HC & Hs_t & Hs_s)".
+        iExists _, _; iFrame.
+        repeat (iSplitL ""; first done).
+        (iSplitR ""; last done).
+
+        iApply (uval_rel_implies_obs_val with "Hv'"). }
+
+      (* Internal call case *)
+      { apply lookup_defn_cons_Some in Hs.
+        destruct Hs.
+        (* It is the [e_s] function (the hole) *)
+        { destruct H2; inv H2; subst. cbn -[denote_function].
+          iDestruct (dval_rel_inj with "Hdv Hmain") as %Hdef; subst.
+          destruct (RelDec.rel_dec (DVALUE_Addr main) (DVALUE_Addr main))
+            eqn: Hf; reldec; subst; last done.
+          rewrite /fun_logrel.
+          iDestruct "HWF" as %HWF.
+          iDestruct ("Hf" $! _ _ _) as "(_ & Hf')".
+
+          iSpecialize ("Hf'" $! _ _ nil nil HWF with "Hst Hss").
+          cbn -[denote_function].
+          iSpecialize ("Hf'" $! Logic.I with "HC").
+
+          iApply sim_expr'_bupd_mono; last (iApply "Hf'").
+          iIntros (??) "H'".
+          rewrite /lift_post.
+          iDestruct "H'" as (????) "(Hs_t & Hs_s & HC & Hval)".
+          iExists _, _; iFrame. subst; iModIntro.
+          repeat (iSplitL ""; first done).
+          (iSplitR ""; last done).
+          iApply (uval_rel_implies_obs_val with "Hval"). }
+
+        (* It is a function in the context *)
+        { destruct H2; cbn -[denote_function].
+
+          iDestruct (dval_rel_ne_inj with "Hdv Hmain") as "%Hne"; subst.
+          specialize (Hne H2); subst.
+          destruct (RelDec.rel_dec (DVALUE_Addr main) dv) eqn: Hf;
+            reldec; subst; first done.
+          clear H2 Hne Hf.
+          iPoseProof (dval_rel_lookup_some with "Hmain Hv") as "%Hlu".
+          specialize (Hlu _ H3). destruct Hlu as (?&?).
+          rewrite /lookup_defn H2.
+
+          (* Juicing out information from the WF of fundefs *)
+          unfold fundefs_WF in WF_s.
+          apply andb_prop_elim in WF_s.
+          destruct WF_s as (Hlen & Wdup_s).
+          apply andb_prop_elim in Hlen. destruct Hlen as (Hlen & Hfun_wf).
+          apply forallb_True in Hfun_wf.
+          rewrite List.Forall_forall in Hfun_wf.
+          assert (Hr_s := H3).
+          apply lookup_defn_Some_In in H3.
+          (* Function [d] is well-formed. *)
+          specialize (Hfun_wf _ H3); cbn in Hfun_wf.
+
+          (* Using [fundefs_logrel] *)
+          assert (Hlen': (length [γf0] > 0)%Z → (length [γf] > 0)%Z) by auto.
+          rewrite /fundefs_logrel.
+          apply lookup_defn_Some_lookup in Hr_s.
+          destruct Hr_s.
+          (* Juice information out of fundef rel WF *)
+          iDestruct "Hrel" as "(Hrel & Hn)".
+          iSpecialize ("Hrel" $! _ _ _ H6).
+          iDestruct "Hrel" as (???)
+                                "(#Hdv' & %Hattr & %Hattr' & %Hft & %Hfs)".
+
+          iSpecialize ("Hlr" $! _ _ _ _ _ _ H7 H6 Hattr Hattr'
+                        with "Hdv'").
+          iSpecialize ("Hlr" $! _ _ nil nil Hlen' with "Hst Hss").
+          cbn -[denote_function].
+          iSpecialize ("Hlr" $! Logic.I with "HC").
+
+          iDestruct (dval_rel_inj with "Hmain Hdv'") as %Hf; subst.
+
+          eapply lookup_defn_Some in H2; eauto;cycle 1.
+          { clear -WF_t.
+
+            unfold fundefs_WF in WF_t.
+            apply andb_prop_elim in WF_t.
+            destruct WF_t as (Hlen & Wdup_t).
+            apply andb_prop_elim in Hlen. destruct Hlen as (Hlen & Hfun_wf).
+            apply forallb_True in Hfun_wf.
+            rewrite List.Forall_forall in Hfun_wf.
+            apply Is_true_true_1 in Wdup_t.
+            by apply NoDup_b_NoDup. }
+          eauto.
+          subst.
+
+          iApply sim_expr'_bupd_mono; last iApply "Hlr".
+          iIntros (??) "Hin".
+          iDestruct "Hin" as (????) "(Hst & Hss & HC & Hval)".
+          iExists _, _; subst.
+          repeat (iSplitL ""; first done); iFrame.
+          (iSplitR ""; last done).
+
+          iApply (uval_rel_implies_obs_val with "Hval"). } } }
+      Unshelve.
+      all : eauto. all: do 2 constructor.
+    Qed.
+
+
+      { cbn.
+
+
+    Admitted.
+
+  End mcfg_contextual.
